lib/FiniteMaps.v
@@ -18,13 +18,13 @@ Module FiniteMap (I : INDEXED_TYPE).
     PTree.fold_spec PTree.fold1_spec.
 
   Local Hint Resolve I.index_inj.
-  
+
   Definition elt    : Type                                 := I.t.
   Definition elt_eq : forall a b : elt, {a = b} + {a <> b} := I.eq.
-  
+
   Definition t     : Type -> Type         := PTree.t.
   Definition empty : forall A : Type, t A := PTree.empty.
-  
+
   Definition get    (A : Type) : elt ->      t A -> option A :=
     @PTree.get    A ∘ I.index.
   Definition set    (A : Type) : elt -> A -> t A -> t A      :=
@@ -34,7 +34,7 @@ Module FiniteMap (I : INDEXED_TYPE).
 
   Definition filter (A : Type) (p : A -> bool) : t A -> t A :=
     PTree.filter1 p.
-  
+
   Local Ltac basic :=
     simpl in *;
     repeat unfold elt, elt_eq,
@@ -51,23 +51,23 @@ Module FiniteMap (I : INDEXED_TYPE).
     eauto.
 
   (* Basic tree properties: empty, get, set, and remove *)
-  
+
   Theorem gempty : forall (A : Type) (i : elt),
     get i (empty A) = None.
   Proof. basic. Qed.
-    
+
   Theorem gss : forall (A : Type) (i : elt) (x : A) (m : t A),
     get i (set i x m) = Some x.
   Proof. basic. Qed.
-  
+
   Theorem gso : forall (A : Type) (i j : elt) (x : A) (m : t A),
     i <> j -> get i (set j x m) = get i m.
   Proof. basic. Qed.
-  
+
   Theorem gsspec : forall (A : Type) (i j : elt) (x : A) (m : t A),
     get i (set j x m) = if elt_eq i j then Some x else get i m.
   Proof. basic. Qed.
-    
+
   Theorem gsident : forall (A : Type) (i : elt) (m : t A) (v : A),
     get i m = Some v -> set i v m = m.
   Proof. basic. Qed.
@@ -75,11 +75,11 @@ Module FiniteMap (I : INDEXED_TYPE).
   Theorem grs : forall (A : Type) (i : elt) (m : t A),
     get i (remove i m) = None.
   Proof. basic. Qed.
-  
+
   Theorem gro : forall (A : Type) (i j : elt) (m : t A),
     i <> j -> get i (remove j m) = get i m.
   Proof. basic. Qed.
-  
+
   Theorem grspec : forall (A : Type) (i j : elt) (m : t A),
     get i (remove j m) = if elt_eq i j then None else get i m.
   Proof. basic. Qed.
@@ -87,12 +87,12 @@ Module FiniteMap (I : INDEXED_TYPE).
   Theorem gfilter {V} : forall (f : V -> bool) (m : t V) (k : elt),
                           get k (filter f m) = option_filter f (get k m).
   Proof. intros. apply PTree.gfilter1. Qed.
-  
+
   (* Equality *)
-  
+
   Definition beq : forall A : Type, (A -> A -> bool) -> t A -> t A -> bool :=
     PTree.beq.
-  
+
   Theorem beq_sound : forall (A : Type) (eqA : A -> A -> bool) (m1 m2 : t A),
     beq eqA m1 m2 = true ->
     (forall (x : elt), match get x m1, get x m2 with
@@ -105,29 +105,29 @@ Module FiniteMap (I : INDEXED_TYPE).
     basic; rewrite PTree.beq_correct in Hbeq; specialize Hbeq with (I.index x).
     assumption.
   Qed.
-  
+
   (* Mapping *)
-  
+
   Definition map1 : forall A B : Type, (A -> B) -> t A -> t B := PTree.map1.
-  
+
   Theorem gmap1 : forall (A B : Type) (f : A -> B) (i : elt) (m : t A),
     get i (map1 f m) = option_map f (get i m).
   Proof. basic. Qed.
 
   (* Combining *)
-  
+
   Definition combine : forall A B C : Type,
                          (option A -> option B -> option C) ->
                          t A -> t B -> t C :=
     PTree.combine.
-  
+
   Theorem gcombine : forall (A B C : Type)
                             (f : option A -> option B -> option C),
     f None None = None ->
     forall (m1 : t A) (m2 : t B) (i : elt),
       get i (combine f m1 m2) = f (get i m1) (get i m2).
   Proof. basic. Qed.
-  
+
   Theorem combine_commut : forall (A B : Type)
                                   (f g : option A -> option A -> option B),
     (forall (i j : option A), f i j = g j i) ->
@@ -143,13 +143,13 @@ Module FiniteTotalMap (I : INDEXED_TYPE) <: MAP.
   Local Hint Resolve I.index_inj.
   Definition elt    : Type                                 := I.t.
   Definition elt_eq : forall a b : elt, {a = b} + {a <> b} := I.eq.
-  
+
   Definition t    : Type -> Type              := PMap.t.
   Definition init : forall A : Type, A -> t A := PMap.init.
-  
+
   Definition get (A : Type) : elt ->      t A -> A   := @PMap.get A ∘ I.index.
   Definition set (A : Type) : elt -> A -> t A -> t A := @PMap.set A ∘ I.index.
-  
+
   Local Ltac basic :=
     simpl in *;
     repeat unfold elt, elt_eq,
@@ -164,9 +164,9 @@ Module FiniteTotalMap (I : INDEXED_TYPE) <: MAP.
     end;
     repeat subst;
     eauto.
-  
+
   (* Basic map properties: init, get, and set *)
-  
+
   Theorem gi : forall (A : Type) (i : elt) (x : A),
     get i (init x) = x.
   Proof. basic. Qed.
@@ -190,7 +190,7 @@ Module FiniteTotalMap (I : INDEXED_TYPE) <: MAP.
   Theorem set2: forall (A : Type) (i : elt) (x y : A) (m : t A),
     set i y (set i x m) = set i y m.
   Proof. basic; eauto using PMap.set2. Qed.
-  
+
   (* Mapping *)
 
   Definition map : forall A B : Type, (A -> B) -> t A -> t B := PMap.map.
@@ -210,10 +210,10 @@ Module NIndexed := NIndexed.
 
 Module PositiveIndexed <: INDEXED_TYPE.
   Definition t := positive.
-  
+
   Definition index := @id positive.
   Arguments index /.
-  
+
   Theorem index_inj : forall x y : positive, index x = index y -> x = y.
   Proof. auto. Qed.
 
@@ -223,11 +223,11 @@ End PositiveIndexed.
 
 Module NatIndexed <: INDEXED_TYPE.
   Definition t := nat.
-  
+
   Definition index := Pos.of_nat ∘ S.
   Arguments index x /.
   Local Arguments Pos.of_nat n : simpl nomatch.
-  
+
   Theorem index_inj : forall x y : nat, index x = index y -> x = y.
   Proof.
     simpl; intros x y Heq; apply Nat2Pos.inj in Heq;
@@ -238,27 +238,26 @@ Module NatIndexed <: INDEXED_TYPE.
   Arguments eq_nat_dec /.
 End NatIndexed.
 
-Require Integers.
+Require Import Integers.
 
-Module IntIndexed (WS : Integers.WORDSIZE) <: INDEXED_TYPE.
-  Module Int := Integers.Make WS.
-  Import Int.
-  
-  Definition t := int.
-  
-  Definition index := ZIndexed.index ∘ intval.
+Module IntIndexed (WS : WORDSIZE) <: INDEXED_TYPE.
+  Import WS.
+
+  Definition t := Word.int wordsize_minus_one.
+
+  Definition index : t -> positive := ZIndexed.index ∘ Word.unsigned.
   Arguments index x /.
-  
-  Lemma intval_inj : forall x y : int, intval x = intval y -> x = y.
+
+  Lemma intval_inj : forall x y : t, Word.unsigned x = Word.unsigned y -> x = y.
   Proof.
-    intros x y Hix; generalize (eq_spec x y); intros Heq.
-    unfold eq, unsigned in *.
+    intros x y Hix; generalize (Word.eq_spec _ x y); intros Heq.
+    unfold Word.eq, Word.unsigned in *.
     rewrite Hix, zeq_true in Heq.
     exact Heq.
   Qed.
-  
-  Theorem index_inj : forall x y : int, index x = index y -> x = y.
+
+  Theorem index_inj : forall x y, index x = index y -> x = y.
   Proof. auto using intval_inj, ZIndexed.index_inj. Qed.
 
-  Definition eq : forall x y : int, {x = y} + {x <> y} := eq_dec.
+  Definition eq : forall x y : t, {x = y} + {x <> y} := Word.eq_dec.
 End IntIndexed.
